Working on FSM, implemented some basic monads.

main.ml
@@ -21,7 +21,7 @@ let implode l =
 
 let str_to_list (s : string) : char list = explode s
 let list_to_str (l : char list) : string = implode l
-let fail message = Printf.printf "%s\n" message; exit 1
+let fail message = Printf.eprintf "%s\n" message; exit 1
 
 type transfer_direction = Upload of string | Download of string
 
@@ -30,11 +30,11 @@ let parse_args () =
   let port = ref 69 in
   let upload = ref "" in
   let download = ref "" in
-  Arg.parse [("-ip", Arg.Set_string ip, "IP address of server to connect to"); ("-port", Arg.Set_int port, "port of the server"); ("-download", Arg.Set_string download, "filename to download"); ("-upload", Arg.Set_string upload, "filename to upload")] (fun anon -> Printf.printf "Unrecognized argument: %s\n" anon; exit 1) "Simple TFTP client in OCaml and Coq";
+  Arg.parse [("-ip", Arg.Set_string ip, "IP address of server to connect to"); ("-port", Arg.Set_int port, "port of the server"); ("-download", Arg.Set_string download, "filename to download"); ("-upload", Arg.Set_string upload, "filename to upload")] (fun anon -> Printf.eprintf "Unrecognized argument: %s\n" anon; exit 1) "Simple TFTP client in OCaml and Coq";
   if !ip = "" then fail "IP not specified";
   if !upload = "" && !download = "" then fail "Provide a filename to download or upload";
   if !upload <> "" && !download <> "" then fail "You can either choose download or upload but not both";
-  if !upload != "" then (!ip, !port, Upload !upload)
+  if !upload <> "" then (!ip, !port, Upload !upload)
   else (!ip, !port, Download !download)
 
 let assign_random_TID () : int =
@@ -53,20 +53,23 @@ let create_udp_socket (tid : int) : file_descr =
 
 type state = TFTP_Core.state
 type message = bytes
-type action = Send of message * int | Terminate
+type action = Send of message * int | Terminate | Continue
 type event = Incoming of message * int | Timeout (* TODO should also provide IP? *) (*TODO add terminated event*)
 
-let translate_coq_result (coq_action, coq_state) : action * state =
+let translate_coq_result (coq_state, coq_action) : action * state =
   let action = match coq_action with
     | Coq_send (msg, port) -> Send (list_to_str msg, port)
-    | Coq_terminate -> Terminate in
+    | Coq_terminate -> Terminate
+    | Coq_continue -> Continue
+  in
   (action, coq_state)
 
 let initialize_connection (tid : int) (port : int) (transfer : transfer_direction) : action * state =
   let coq_transfer = match transfer with
-    | Upload fname -> TFTP_Core.Coq_upload (str_to_list fname)
-    | Download fname -> TFTP_Core.Coq_download (str_to_list fname)
+    | Upload fname -> fail "Upload is not implemented"
+    | Download fname -> str_to_list fname
   in
+  (* let init_state = TFTP_Core.initial_state in *)
   translate_coq_result (TFTP_Core.initialize tid port coq_transfer)
 
 let process_step (event :  event) (state : state) : action * state =
@@ -79,21 +82,15 @@ let max_packet_len = 600
 
 let main =
   Random.self_init(); (* initialize randomness *)
-  Printf.printf "hello world\n";
+  Printf.eprintf "hello world\n";
   let (ip, port, transfer) = parse_args() in
   let tid = assign_random_TID () in
-  Printf.printf "Connecting to %s:%d, my tid is %d\n%!" ip port tid;
+  Printf.eprintf "Connecting to %s:%d, my tid is %d\n%!" ip port tid;
   let fd = create_udp_socket tid in
   let make_addr port = ADDR_INET ((inet_addr_of_string ip), port) in
-  let rec loop (action, state) =
-    match action with
-    | Terminate -> Printf.printf "quitting\n"; exit 0
-    | Send (msg, port) ->
-      Printf.printf "sending '%s'\n%!" (Bytes.to_string msg);
-      let toaddr = make_addr port in
-      let sent = Unix.sendto fd msg 0 (Bytes.length msg) [] toaddr in
-      if sent <> Bytes.length msg then Printf.printf "Warning: message has not been sent whole, shouldn't ever happen with UDP! Sent %d/%d bytes" sent (Bytes.length msg);
-      Printf.printf "waiting for reply\n%!";
+  let rec
+    receive state =
+      Printf.eprintf "waiting for reply\n%!";
       let buf = Bytes.create max_packet_len in
       try
         let (recvd, sender) = Unix.recvfrom fd buf 0 max_packet_len [] in
@@ -101,13 +98,24 @@ let main =
         | ADDR_UNIX _ -> fail "Did not expect a UNIX message on UDP socket!"
         | ADDR_INET (fromip, fromport) ->
           if recvd <= 0 then (* TODO this is not a timeout but terminated conn *)
-            (Printf.printf "Receive error\n%!";
+            (Printf.eprintf "Receive error\n%!";
             loop (process_step Timeout state))
           else
-            (Printf.printf "received '%s'\n%!" (Bytes.to_string buf);
+            (Printf.eprintf "received '%s' from %d\n%!" (escaped (Bytes.to_string buf)) fromport;
             loop (process_step (Incoming (Bytes.sub buf 0 recvd, fromport)) state))
       with Unix.Unix_error (Unix.EAGAIN, "recvfrom", _) ->
-        Printf.printf "Timed out\n%!";
+        Printf.eprintf "Timed out\n%!";
         loop (process_step Timeout state)
+    and
+    loop (action, state) =
+    match action with
+    | Continue -> receive state
+    | Terminate -> Printf.eprintf "quitting\n"; exit 0
+    | Send (msg, port) ->
+      Printf.eprintf "sending '%s' to %d\n%!" (escaped (Bytes.to_string msg)) port;
+      let toaddr = make_addr port in
+      let sent = Unix.sendto fd msg 0 (Bytes.length msg) [] toaddr in
+      if sent <> Bytes.length msg then Printf.eprintf "Warning: message has not been sent whole, shouldn't ever happen with UDP! Sent %d/%d bytes" sent (Bytes.length msg);
+      receive state
   in
   loop (initialize_connection tid port transfer)
